feat: rework StrongBisim definition to use inductive
The idea is that this helps remove a bunch of inversion lemmas,
since we can now directly match on the inductive proposition.

In practice, since the inductive proposition is always over a
function application in its index, we need to generalize it
before we can proceed with the pattern matching. To aid in its
use, we give a `StrongBisim.cases` auxiliary theorem which
helps to automatically generalize the indices.

It might be worth it to consider changing the inductive
proposition so matching over it is easier, but the current
solution simplifies sufficiently the proofs.

IterTree/Basic.lean
@@ -151,52 +151,24 @@ inductive Obs (E : Type q → Type r) (R : Type v) (K : Type k) where
 | tau : K → Obs E R K
 | vis {A : Type q} : E A → (A → K) → Obs E R K
 
+@[simp, grind]
 def Obs.mapState (f : α → β) : Obs E R α → Obs E R β
 | .ret v => .ret v
 | .tau st => .tau <| f st
 | .vis ev k => .vis ev (fun x => f (k x))
 
+@[simp, grind]
 def Obs.bindVal (f : α → Obs E β K) : Obs E α K → Obs E β K
 | .ret v => f v
 | .tau st => .tau st
 | .vis ev k => .vis ev k
 
 
-/- class IsITreeImpl (State : Type s) (E : Type q → Type r) (R : Type v) where -/
-/-     step : State → Obs E R State -/
-
 structure iTree (E : Type q → Type r) (R : Type v) where
-  {State : Type s} -- TODO: Maybe rename to MetaState
+  {State : Type s}
   curr : State
-  /- [stepImpl : IsITreeImpl State E R] -/
   step : State → Obs E R State
 
-  -- Why not have it give observations on just `State`?
-  -- I think it's not possible, because we must be able to change
-  -- the state type at some point in the execution.
-  --
-  -- However, how do you define the infinitely looping
-  -- computation with `State → Obs E R (iTree E R)`?
-  -- You can't, you'd need to reference back to the think you're
-  -- defining, but at that point it's no longer a fixpoint!
-
-  -- In short, it can't be State → Obs E R (iTree E R) because
-  -- then one can't really give an infinitely looping computation
-  -- It also can't be `State → Obs E R State` because one should
-  -- be able to encode that the state changes from one computation
-  -- to another. Or can't it?
-  --
-  -- The issue with doing this encoding is that one must fix the
-  -- type of the state of the final computation, but it's not
-  -- trivial to define. For instance, one would like to say that
-  -- when doing a `bind` with `f`, the state will originally be
-  -- that of the interaction tree being executed, until it gives
-  -- a value `a`, at which point one switches to the state of the
-  -- `iTree` resulting from applying `f` to `a`. However, this
-  -- cannot be expressed directly as a type.
-  -- One could, however, express this as an invariant of the
-  -- structure, which leads us back to the `IsPlausibleStep` of
-  -- `Std.Iter`.
 /-
 
 An alternate representation of this interface would be to have `curr : State` be the implementation of
@@ -222,21 +194,15 @@ def unfold (it : iTree E R) : Obs E R (iTree E R) :=
   | .tau next => .tau {it with curr := next}
   | .vis ev k => .vis ev (fun x => {it with curr := (k x)})
 
-theorem unfold_cases (it : iTree E R) :
-    (∃ v, it.unfold = .ret v) ∨
-    (∃ (α : Type _) (ev : E α) (k : α → iTree E R), it.unfold = .vis ev k) ∨
-    (∃ it', it.unfold = .tau it') :=
-  match it.unfold with
-  | .ret v => .inl ⟨v, rfl⟩
-  | .vis (A := α) ev k => .inr <| .inl ⟨α, ev, k, rfl⟩
-  | .tau next => .inr <| .inr ⟨next, rfl⟩
+/- theorem unfold_cases (it : iTree E R) : -/
+/-     (∃ v, it.unfold = .ret v) ∨ -/
+/-     (∃ (α : Type _) (ev : E α) (k : α → iTree E R), it.unfold = .vis ev k) ∨ -/
+/-     (∃ it', it.unfold = .tau it') := -/
+/-   match it.unfold with -/
+/-   | .ret v => .inl ⟨v, rfl⟩ -/
+/-   | .vis (A := α) ev k => .inr <| .inl ⟨α, ev, k, rfl⟩ -/
+/-   | .tau next => .inr <| .inr ⟨next, rfl⟩ -/
 /- grind_pattern unfold_cases => it.unfold -/
--- NOTE: It might be enough with [grind cases] on `Obs`.
-
--- Maybe this can be defined later, once we have equality over unfoldings.
-/- def recUnfold {motive : iTree E R → Prop} -/
-/-   (onRet : (v : R) → motive (.ret v)) -/
-/-   (onTau : (it iTree E R → -/
 
 def ret.{s} (r : R) : iTree E R where
   curr : PUnit.{s+1}  := .unit
@@ -247,12 +213,6 @@ def vis.{s} {α : Type q} (ev : E α) (k : α → iTree.{_,_,_,s} E R) : iTree E
   step
   | .inl .unit => .vis ev (fun a => .inr <| ⟨a, (k a).curr⟩)
   | .inr ⟨a, s⟩ => (k a).step s |>.mapState (.inr ⟨a, ·⟩)
-  -- TODO: I could probably generalize this structure of
-  -- "stay in inl until something, then inr always", and
-  -- prove some generic lemmas about it, to reduce the proof
-  -- burden.
-  -- Would also be cool to state that "once a is chosen, it
-  -- doesn't change"
 
 def tau.{s} (it : iTree.{_,_,_,s} E R) : iTree E R where
   -- We basically generate an artificial prior element in the state.
@@ -267,7 +227,6 @@ def Obs.toITree : Obs E R (iTree E R) → iTree E R
 | .tau it => iTree.tau it
 | .vis ev k => iTree.vis ev k
 | .ret v => iTree.ret v
-
 
 namespace iTree
 
@@ -489,8 +448,11 @@ coinductive_fixpoint monotonicity fun r r' himp => by
 end SecondTry
 
 namespace ThirdTry
-variable {E : Type quest → Type resp}{R : Type ret}
 
+local instance : Std.Refl (Eq (α := α)) where refl := .refl 
+local instance : Std.Symm (Eq (α := α)) where symm _ _:= .symm
+
+variable {E : Type quest → Type resp}{R : Type ret}
 
 /-
 
@@ -498,274 +460,172 @@ We define a weaker version of equality, observational
 
 -/
 
--- TODO: Maybe it'd be cool to define it as a mutually recursive relation.
--- where we have relatiosn between Obs E R (iTree E R) and iTree E R defined
--- in terms of one another.
--- Might be useful for grind lemmas.
-
-mutual
-  -- Eqit (r : R → R → Prop) (l r : Bool) [i.e. eutt :0 Eqit (· = ·) true true]
-  abbrev Rel (r : R → R → Prop) (it₁ it₂ : iTree E R)  : Prop := ObsRel r it₁.unfold it₂.unfold
-  coinductive_fixpoint monotonicity by
-    rintro Rel Rel' ⟨_, Obsimp⟩ it₁ it₂ H
-    apply Obsimp
-    assumption
-
-  def ObsRel (r : R → R → Prop) : Obs E R (iTree E R) → Obs E R (iTree E R) → Prop
-  | .ret v₁, .ret v₂ =>
-      r v₁ v₂
-  | .vis (A := A₁) ev₁ k₁, .vis (A := A₂) ev₂ k₂ =>
-      ∃ (h : A₁ = A₂), ev₁ = h ▸ ev₂ ∧ ∀ s₁,
-        Rel r (k₁ s₁) (k₂ (h ▸ s₁))
-  | .tau it₁', .tau it₂' =>
-      Rel r it₁' it₂'
-  | _, _ => False
-  coinductive_fixpoint monotonicity by
-    rintro ⟨Rel, Obs⟩ ⟨Rel', Obs'⟩ ⟨Rimp, _⟩ obs₁ obs₂ H
-    match h₁ : obs₁ with
-    | .ret v₁ =>
-        cases h₂ : obs₂ <;> grind
-    | .vis (A := A₁) ev₁ k₁ =>
-        match obs₂ with
-        | .ret v₂ => grind
-        | .tau it₂ => grind
-        | .vis (A := A₂) ev₂ k₂ =>
-          obtain ⟨h, rfl, ext⟩ := H
-          simp only [Lean.Order.PartialOrder.rel, true_and, h, exists_true_left] at *
-          intros; apply Rimp; apply ext
-    | .tau it₁ =>
-        match  obs₂ with
-        | .ret v₂ => grind
-        | .vis (A := A₂) ev₂ k₂ => grind
-        | .tau it₂ =>
-          apply Rimp
-          assumption
-
-end
-
-
 --- lift (?). Maybe with `postFix`? ObsRelF? `eqitF` maybe
 -- coinduction template
-abbrev ObsRel.func (s : iTree E R → iTree E R → Prop) (r : R → R → Prop) : Obs E R (iTree E R) → Obs E R (iTree E R) → Prop
-| .ret v₁, .ret v₂ =>
-    r v₁ v₂
-| .vis (A := A₁) ev₁ k₁, .vis (A := A₂) ev₂ k₂ =>
-    ∃ (h : A₁ = A₂), ev₁ = h ▸ ev₂ ∧ ∀ s₁,
-      s (k₁ s₁) (k₂ (h ▸ s₁))
-| .tau it₁', .tau it₂' =>
-    s it₁' it₂'
-| _, _ => False
 
-/- def ObsRel (r : R → R → Prop)(it₁ it₂ : iTree E R) : Prop := -/
-/-   match it₁.unfold, it₂.unfold with -/
-/-   | .ret v₁, .ret v₂ => -/
-/-       r v₁ v₂ -/
-/-   | .vis (A := A₁) ev₁ k₁, .vis (A := A₂) ev₂ k₂ => -/
-/-       ∃ (h : A₁ = A₂), ev₁ = h ▸ ev₂ ∧ ∀ s₁, -/
-/-         ObsRel r (k₁ s₁) (k₂ (h ▸ s₁)) -/
-/-   | .tau it₁', .tau it₂' => -/
-/-       ObsRel r it₁' it₂' -/
-/-   | _, _ => False -/
-/- coinductive_fixpoint monotonicity fun ObsRel ObsRel' Himp it₁ it₂ H => by -/
-/-   dsimp at H ⊢ -/
-/-   match h₁ :  it₁.unfold with -/
-/-   | .ret v₁ => -/
-/-       simp [h₁] at H ⊢ -/
-/-       cases h₂ : it₂.unfold <;> grind -/
-/-   | .vis (A := A₁) ev₁ k₁ => -/
-/-       simp [h₁] at H ⊢ -/
-/-       match h₂ : it₂.unfold with -/
-/-       | .ret v₂ => grind -/
-/-       | .tau it₂ => grind -/
-/-       | .vis (A := A₂) ev₂ k₂ => -/
-/-         simp [h₂] at H ⊢ -/
-/-         obtain ⟨h, rfl, ext⟩ := H -/
-/-         subst h -/
-/-         simp -/
-/-         intros -/
-/-         apply Himp -/
-/-         apply ext -/
-/-   | .tau it₁ => -/
-/-       simp [h₁] at H ⊢ -/
-/-       match h₂ : it₂.unfold with -/
-/-       | .ret v₂ => grind -/
-/-       | .vis (A := A₂) ev₂ k₂ => grind -/
-/-       | .tau it₂ => -/
-/-         simp [h₂] at H ⊢ -/
-/-         apply Himp -/
-/-         assumption -/
+inductive RelOverObs (s : S₁ → S₂ → Prop) (r : R → R → Prop) : 
+    Obs E R S₁ → Obs E R S₂ → Prop where
+  | ret (v₁ v₂ : R) : r v₁ v₂ → RelOverObs s r (.ret v₁) (.ret v₂)
+  | tau (it₁ : S₁) (it₂ : S₂) : s it₁ it₂ → RelOverObs s r (.tau it₁) (.tau it₂)
+  | vis (A : Type _) (ev : E A) (k₁ : A → S₁) (k₂ : A → S₂) :
+    (∀ x, s (k₁ x) (k₂ x)) → RelOverObs s r (.vis ev k₁) (.vis ev k₂)
 
-abbrev ObsEq (it₁ it₂ : iTree E R) := Rel (· = ·) it₁ it₂
+/- @[simp] -/
+/- abbrev relOverObs (s : iTree E R → iTree E R → Prop) (r : R → R → Prop) : Obs E R (iTree E R) → Obs E R (iTree E R) → Prop -/
+/- | .ret v₁, .ret v₂ => r v₁ v₂ -/
+/- | .tau it₁', .tau it₂' => s it₁' it₂' -/
+/- | .vis (A := A₁) ev₁ k₁, .vis (A := A₂) ev₂ k₂ => -/
+/-     ∃ (h : A₁ = A₂), ev₁ = h ▸ ev₂ ∧ ∀ s₁, -/
+/-       s (k₁ s₁) (k₂ (h ▸ s₁)) -/
+/- | _, _ => False -/
 
-abbrev ObsEq.func s (obs₁ obs₂ : Obs E R (iTree E R)) := ObsRel.func s (·=·) obs₁ obs₂
-
-instance {E : Type _ → Type _} : HasEquiv (iTree E R) where
-  Equiv := ObsEq
-
-/- @[grind →] -/
-/- theorem ObsEq.cases (it₁ it₂ : iTree E R) : -/
-/-     it₁ ≈ it₂ → -/
-/-     (∃ v₁, it₁.unfold = .ret v₁) ∧ (∃ v₂, it₂.unfold = .ret v₂) ∨ -/
-/-     (∃ (A₁ : Type) (ev₁ : E A₁) (k₁ : A₁ → iTree E R), it₁.unfold = .vis ev₁ k₁) ∧ -/
-/-     (∃ (A₂ : Type) (ev₂ : E A₂) (k₂ : A₂ → iTree E R), it₂.unfold = .vis ev₂ k₂) ∨ -/
-/-     (∃ it₁', it₁.unfold = .tau it₁') ∧ (∃ it₂', it₂.unfold = .tau it₂') := fun h => -/
-/-   match h₁ : it₁.unfold, h₂ : it₂.unfold with -/
-/-   | .ret v₁, .ret v₂ => by grind -/
-/-   | .vis (A := A₁) ev₁ k₁, .vis (A := A₂) ev₂ k₂ => by grind -/
-/-   | .tau it₁', .tau it₂' => by grind -/
-/-   | .ret .., .tau .. -/
-/-   | .ret .., .vis .. -/
-/-   | .vis .., .ret .. -/
-/-   | .vis .., .tau .. -/
-/-   | .tau .., .vis .. -/
-/-   | .tau .., .ret .. => by simp only [h₁, h₂, ObsRel] at h -/
-
-@[grind →]
-theorem ObsEq.obsEq_unfold_eq_ret {it₁ it₂ : iTree E R} :
-    it₁.unfold = .ret v₁ →
-    it₁ ≈ it₂ →
-    ∃ v₂, it₂.unfold = .ret v₂ := fun h₁ h => by
-  unfold Rel at h
-  cases h₂ : it₂.unfold <;> simp [h₁, h₂, ObsRel] at h
-  case ret v₂ => exists v₂
-
-@[grind →]
-theorem ObsEq.obsEq_unfold_eq_vis {it₁ it₂ : iTree E R} {ev₁ : E A₁} {k₁} :
-    it₁.unfold = .vis ev₁ k₁ →
-    it₁ ≈ it₂ →
-    ∃ (A₂ : Type _) (ev₂ : E A₂) (k₂ : A₂ → iTree E R), it₂.unfold = .vis ev₂ k₂ := fun h₁ h => by
-  unfold Rel at h
-  cases h₂ : it₂.unfold <;> simp [h₁, h₂, ObsRel] at h
-  case vis A₂ ev₂ k₂ => exists A₂, ev₂, k₂
-
-@[grind →] -- Inversion lemmas (`_inv`)
-theorem ObsEq.obsEq_unfold_eq_tau {it₁ it₂ it₁' : iTree E R} :
-    it₁.unfold = .tau it₁' →
-    it₁ ≈ it₂ →
-    ∃ it₂', it₂.unfold = .tau it₂' := fun h₁ h => by
-  unfold Rel at h
-  cases h₂ : it₂.unfold <;> simp [h₁, h₂, ObsRel] at h
-  case tau it₂ => exists it₂
-
-theorem ObsEq.unfold_eq_ret {it₁ it₂ : iTree E R} {v₁ : R} {v₂ : R} :
-    it₁.unfold = .ret v₁ →
-    it₂.unfold = .ret v₂ →
-    it₁ ≈ it₂ →
-    v₁ = v₂ := fun h₁ h₂ h => by
-  unfold Rel at h
-  simpa [h₁, h₂, ObsRel] using h
-
-theorem ObsEq.unfold_eq_vis {it₁ it₂ : iTree E R} {ev₁ : E A₁} {ev₂ : E A₂} {k₁ k₂} :
-    it₁.unfold = .vis ev₁ k₁ →
-    it₂.unfold = .vis ev₂ k₂ →
-    it₁ ≈ it₂ →
-    ∃ (h : A₁ = A₂), ev₁ = h ▸ ev₂ ∧ ∀ s₁,
-      (k₁ s₁) ≈ (k₂ (h ▸ s₁)) := fun h₁ h₂ h => by
-  unfold Rel at h
-  simpa [h₁, h₂, ObsRel] using h
-
-theorem ObsEq.unfold_eq_tau {it₁ it₂ it₁' : iTree E R} :
-    it₁.unfold = .tau it₁' →
-    it₂.unfold = .tau it₂' →
-    it₁ ≈ it₂ →
-    it₁' ≈ it₂' := fun h₁ h₂ h => by
-  unfold Rel at h
-  simpa [h₁, h₂, ObsRel] using h
-
-@[grind =, grind =_]
-theorem ObsRel.iff_rel {it₁ it₂ : iTree E R} :
-    it₁ ≈ it₂ ↔ ObsRel (·=·) it₁.unfold it₂.unfold := by
-  unfold Rel
-  exact ⟨id, id⟩
-
-#check Rel.coinduct
-#print ObsRel.func
-
--- parametrized coinduction (what rocq-paco does, actually)
-def ObsEq.coinductWith
-  (pred : iTree E R → iTree E R → Prop)
-  {it₁ it₂ : iTree E R}
-  (baseCase : pred it₁ it₂)
-  (progress :
-    ∀ (it₁ it₂ : iTree E R),
-      pred it₁ it₂ → ObsEq.func pred it₁.unfold it₂.unfold) :
-    ObsEq it₁ it₂ := by
-  apply Rel.coinduct (·=·) (pred_1 := pred) (pred_2 := ObsEq.func pred) _ _ _ _ baseCase
-  all_goals grind only
+theorem RelOverObs.mono (s s' : S₁ → S₂ → Prop) (r r' : R → R → Prop) : 
+    (∀ {i i'}, s i i' → s' i i') →
+    (∀ {v v'}, r v v' → r' v v') →
+     ∀ o (o' : Obs E R S₂), (RelOverObs s r) o o' → (RelOverObs s' r') o o' := 
+  fun ss' rr' _ _ => fun
+    | .ret v₁ v₂ h => .ret v₁ v₂ (rr' h)
+    | .tau it₁ it₂ h => .tau _ _ (ss' h)
+    | .vis A ev k₁ k₂ h => .vis A ev k₁ k₂ (ss' <| h ·)
 
 @[refl]
-theorem ObsEq.refl {it : iTree E R} : it ≈ it := by
-  apply ObsEq.coinductWith (·=·) rfl
-  grind only
+theorem RelOverObs.refl (s : S → S → Prop) (r : R → R → Prop) [Std.Refl s] [Std.Refl r] : 
+    ∀ (o : Obs E R S), (RelOverObs s r) o o
+  | .ret v => .ret v v (Std.Refl.refl v)
+  | .tau it => .tau it it (Std.Refl.refl it)
+  | .vis ev k => .vis _ ev k k (Std.Refl.refl <| k ·)
 
- @[symm]
-theorem ObsEq.symm {it₁ it₂ : iTree E R} : it₁ ≈ it₂ → it₂ ≈ it₁ := by
-  intro h
-  apply ObsEq.coinductWith (pred := fun x y => y ≈ x) h
-  intros it₁ it₂ hyp
-  match h₁ : it₁.unfold, h₂ : it₂.unfold with
-  | Obs.ret _, Obs.ret _ =>
-    grind [ObsEq.unfold_eq_ret]
-  | Obs.vis (A := A₁) ev₁ k₁, Obs.vis (A := A₂) ev₂ k₂ =>
-    grind [ObsEq.unfold_eq_vis]
-  | Obs.tau it₁', Obs.tau it₂' =>
-    grind [ObsEq.unfold_eq_tau]
-  | .ret .., .tau ..
-  | .ret .., .vis ..
-  | .vis .., .ret ..
-  | .vis .., .tau ..
-  | .tau .., .vis ..
-  | .tau .., .ret .. =>
-    unfold Rel at hyp
-    simp [h₁, h₂,  ObsRel] at hyp
+instance [Std.Refl s][Std.Refl r] : Std.Refl (RelOverObs (E := E) (R := R) s r) where refl := .refl s r
 
-theorem ObsEq.trans {it₁ it₂ it₃ : iTree E R} : it₁ ≈ it₂ → it₂ ≈ it₃ → it₁ ≈ it₃ := by
-  intro it12 it23
-  apply ObsEq.coinductWith (pred := fun x z => ∃ y, x ≈ y ∧ y ≈ z) ⟨it₂, it12, it23⟩
-  rintro it₁ it₃ ⟨it₂, it12, it23⟩
-  match h₁ : it₁.unfold, h₃ : it₃.unfold with
-  | Obs.ret _, Obs.ret _ =>
-    grind [ObsEq.unfold_eq_ret]
-  | Obs.vis (A := A₁) ev₁ k₁, Obs.vis (A := A₃) ev₃ k₃ =>
-    grind [ObsEq.unfold_eq_vis]
-  | Obs.tau it₁', Obs.tau it₃' =>
-    unfold func ObsRel.func
-    have ⟨it₂', h₂⟩ := ObsEq.obsEq_unfold_eq_tau h₁ it12
-    have it'12 := ObsEq.unfold_eq_tau h₁ h₂ it12
-    have it'23 := ObsEq.unfold_eq_tau h₂ h₃ it23
-    exists it₂'
-  | .ret .., .tau ..
-  | .ret .., .vis ..
-  | .vis .., .ret ..
-  | .vis .., .tau ..
-  | .tau .., .vis ..
-  | .tau .., .ret .. =>
-    have oit12 := ObsRel.iff_rel.1 it12
-    have oit23 := ObsRel.iff_rel.1 it23
-    grind
+@[symm]
+theorem RelOverObs.symm (s : S → S → Prop) (r : R → R → Prop) [Std.Symm s] [Std.Symm r] {o o' : Obs E R S} : 
+    (RelOverObs s r) o o' → (RelOverObs s r) o' o
+  | .ret v₁ v₂ h => .ret v₂ v₁ (Std.Symm.symm v₁ v₂ h)
+  | .tau it₁ it₂ h => .tau it₂ it₁ (Std.Symm.symm it₁ it₂ h)
+  | .vis A ev k₁ k₂ h => .vis _ ev k₂ k₁ (Std.Symm.symm _ _ <| h ·)
 
-instance : Std.Refl (@ObsEq E R) where refl _ := ObsEq.refl
-instance : Std.Symm (@ObsEq E R) where symm _ _ := ObsEq.symm
-instance : Trans (@ObsEq E R) (@ObsEq E R) (@ObsEq E R) where trans := ObsEq.trans
+instance [Std.Symm s][Std.Symm r] : Std.Symm (RelOverObs (E := E) (R := R) s r) where symm _ _ := .symm s r
+
+theorem RelOverObs.trans 
+  {s₁₂ : S₁ → S₂ → Prop} {s₂₃ : S₂ → S₃ → Prop} {s₁₃ : S₁ → S₃ → Prop}
+  {r : R → R → Prop} 
+  [Trans s₁₂ s₂₃ s₁₃] [Trans r r r] {o₁ o₂ o₃} : 
+    (RelOverObs (E := E) s₁₂ r) o₁ o₂ →
+    (RelOverObs (E := E) s₂₃ r) o₂ o₃ →
+    (RelOverObs (E := E) s₁₃ r) o₁ o₃
+  | .ret v₁ v₂ h₁, .ret _ v₃ h₂ => .ret v₁ v₃ (Trans.trans h₁ h₂)
+  | .tau it₁ it₂ h₁, .tau _ it₃ h₂ => .tau it₁ it₃ (Trans.trans h₁ h₂)
+  | .vis _ ev k₁ k₂ h₁, .vis _ _ _ k₃ h₂  => .vis _ ev k₁ k₃ (λx↦ Trans.trans (h₁ x) (h₂ x))
+
+instance [Trans r r r][Trans s₁₂ s₂₃ s₁₃] :
+    Trans (RelOverObs (E := E) (R := R) s₁₂ r) 
+          (RelOverObs (E := E) (R := R) s₂₃ r) 
+          (RelOverObs (E := E) (R := R) s₁₃ r) where
+  trans x y := .trans x y
+
+-- Eqit (r : R → R → Prop) (l r : Bool) [i.e. eutt :0 Eqit (· = ·) true true]
+abbrev StrongBisim (r : R → R → Prop) (it₁ it₂ : iTree E R)  : Prop := 
+  RelOverObs (StrongBisim r) r it₁.unfold it₂.unfold
+coinductive_fixpoint monotonicity
+  fun Rel Rel' Rimp it₁ it₂ H =>
+  RelOverObs.mono Rel' Rel _ _ (Rimp _ _) id it₁.unfold it₂.unfold H
+
+namespace StrongBisim
+
+def cases {it₁ it₂ : iTree E R} (h : StrongBisim r it₁ it₂) :
+      ∃ obs₁ obs₂, it₁.unfold = obs₁ ∧ it₂.unfold = obs₂ ∧ RelOverObs (StrongBisim r) r obs₁ obs₂ := 
+  ⟨_, _, rfl, rfl, StrongBisim.eq_def .. ▸ h⟩
+
+@[refl]
+theorem refl {it : iTree E R} [Std.Refl r]: StrongBisim r it it  := by
+  apply coinduct r (pred := (· = ·)) ?progress _ _ rfl
+  rintro it₁ it₂ rfl
+  rfl
+
+instance [Std.Refl r] : Std.Refl (StrongBisim (E := E) (R := R) r) where refl _ := StrongBisim.refl
+
+/- #check Classical.indefiniteDescription -/ -- Why do I get this in the error message if I invoke `h.cases` as `StrongBisim.cases`?
+
+@[symm]
+theorem symm {it₁ it₂ : iTree E R} [Std.Symm r]: StrongBisim r it₁ it₂ → StrongBisim r it₂ it₁  := by
+  intro start
+  apply coinduct r (pred := λ x y ↦ StrongBisim r y x) ?_ _ _ start
+  intro it₁ it₂ it₂it₁
+  have ⟨obs₁, obs₂, h₁, h₂, cases⟩ := StrongBisim.cases it₂it₁
+  match cases with 
+  | .ret v₁ v₂ h => 
+    rw [h₁, h₂]; constructor; apply Std.Symm.symm _ _ h
+  | .tau it₁ it₂ h => 
+    rw [h₁, h₂]; constructor; exact h
+  | .vis A ev k₁ k₂ h => 
+    rw [h₁, h₂]; constructor; exact h
+
+theorem trans {it₁ it₂ it₃ : iTree E R} [Trans r r r]: StrongBisim r it₁ it₂ → StrongBisim r it₂ it₃ → StrongBisim r it₁ it₃ := by
+  intro H₁ H₂
+  apply coinduct r (pred := λ x z ↦ ∃ y, StrongBisim r x y ∧StrongBisim r y z) ?_ _ _ ⟨it₂, H₁, H₂⟩
+  intro it₁ it₃ ⟨it₂, it₁it₂, it₂it₃⟩
+  unfold StrongBisim at it₁it₂ it₂it₃
+  generalize h₁ : it₁.unfold = obs₁ at *
+  generalize h₂ : it₂.unfold = obs₂ at *
+  generalize h₃ : it₃.unfold = obs₃ at *
+  match it₁it₂, it₂it₃ with 
+  | .ret v₁ v₂ H₁, .ret _ v₃ H₂ => 
+    constructor; exact Trans.trans H₁ H₂
+  | .tau it₁ it₂ H₁, .tau _ it₃ H₂ => 
+    constructor; exact ⟨it₂, H₁, H₂⟩
+  | .vis A ev k₁ k₂ H₁, .vis _ _ _ k₃ H₂ => 
+    constructor; intro x; exact ⟨k₂ x, H₁ x, H₂ x⟩
+    
+instance [Trans r r r] : Trans (StrongBisim (E := E) (R := R) r) (StrongBisim (E := E) (R := R) r) (StrongBisim (E := E) (R := R) r) where trans := StrongBisim.trans
+
+end StrongBisim
+
+abbrev ObsEq : iTree E R → iTree E R → Prop := StrongBisim (· = ·)
+
+instance : HasEquiv (iTree E R) where
+  Equiv := ObsEq
+
+instance : HasEquiv (Obs E R (iTree E R)) where
+  Equiv := RelOverObs (· ≈ ·) (· = ·)
+
+def ObsEq.coinductOn
+  {it₁ it₂ : iTree E R} 
+  (pred : iTree E R → iTree E R → Prop)
+  (baseCase : pred it₁ it₂)
+  (progress : ∀ (it₁ it₂ : iTree E R), pred it₁ it₂ → RelOverObs pred (· = ·) it₁.unfold it₂.unfold) :
+    it₁ ≈ it₂ := 
+  StrongBisim.coinduct (· = ·) pred progress _ _ baseCase
+
+theorem obsEq_unfold {it it' : iTree E R} : 
+    it ≈ it' ↔ it.unfold ≈ it'.unfold :=
+  ⟨(StrongBisim.eq_def .. |>.mp ·), (StrongBisim.eq_def .. |>.mpr ·)⟩
 
 def ObsEq.step_tau_obsEq_self (it : iTree E R) (s : it.State) c :
-    { {it with curr := c}.tau with curr := .inr s } ≈ {it with curr := s} := by
-  apply ObsEq.coinductWith (fun
+    {it with curr := s} ≈ { {it with curr := c}.tau with curr := .inr s } := by
+  apply coinductOn (fun
     (iTree.mk (State := State₁) curr₁ step₁)
     (iTree.mk (State := State₂) curr₂ step₂) =>
-    ∃ (H : State₁ = (PUnit ⊕ State₂)),
-    curr₁ = H.mpr (Sum.inr curr₂) ∧
-    ∀ (s : State₂),
-    step₁ (H ▸ (.inr s)) = H.symm ▸ (step₂ s).mapState .inr
+    ∃ (mpr : (PUnit ⊕ State₁) → State₂),
+    curr₂ = mpr (Sum.inr curr₁) ∧
+    ∀ (s : State₁),
+    step₂ (mpr (.inr s)) = (step₁ s).mapState (mpr <| .inr ·)
   )
   case baseCase =>
+    simp
+    exists id
     simp [tau, Obs.mapState]
   case progress =>
-    unfold func ObsRel.func unfold
-    rintro ⟨c₁, s₁⟩ ⟨c₂, s₂⟩ ⟨rfl, HC, Hs⟩
-    cases _ : s₁ c₁ <;>
-    cases _ : s₂ c₂ <;>
-    simp [*, Obs.mapState]
+    intro it₁ it₂ ⟨H, HC, Hs⟩
+    cases h : it₁.step it₁.curr <;> simp only [h, unfold, HC, Obs.mapState, Hs]
+    case ret v => 
+      constructor; rfl
+    case tau it => 
+      constructor
+      exists H
+    case vis ev k => 
+      constructor
+      intros
+      exists H
 
 def ObsEq.step_vis_obsEq_self (it : iTree E R) (ev : E A) (kS : A → it.State) (a : A) :
     { curr := kS a, step := it.step : iTree E R} ≈
@@ -774,7 +634,7 @@ def ObsEq.step_vis_obsEq_self (it : iTree E R) (ev : E A) (kS : A → it.State) 
           match x with
           | Sum.inl PUnit.unit => Obs.vis ev fun a => Sum.inr ⟨a, kS a⟩
           | Sum.inr ⟨a, s⟩ => Obs.mapState (fun x => Sum.inr ⟨a, x⟩) (it.step s) } := by
-  apply ObsEq.coinductWith (fun
+  apply coinductOn (fun
     (iTree.mk (State := State₁) curr₁ step₁)
     (iTree.mk (State := State₂) curr₂ step₂) =>
     ∃ (mpr : (PUnit ⊕ (_ : A) × State₁) → State₂),
@@ -786,108 +646,35 @@ def ObsEq.step_vis_obsEq_self (it : iTree E R) (ev : E A) (kS : A → it.State) 
     exists id
     simp [Obs.mapState]
   case progress =>
-    rintro ⟨c₁, s₁⟩ ⟨c₂, s₂⟩ ⟨h, HC, Hs⟩
-    unfold ObsEq.func ObsRel.func unfold
-    cases _ : s₁ c₁ <;>
-    cases _ : s₂ c₂ <;>
-    simp [*, Obs.mapState]
-    all_goals (intros; exists h)
-
-/- def ObsEq.step_vis_obsEq_self {E : Type _ → Type _}(ev : E A) (k : A → S) (a : A) (s : S) c : -/
-    /- { iTree.vis ev (fun a => ⟨c, k a⟩) with curr := .inr ⟨a, s⟩ } ≈ {it with curr := s} := by -/
-  /- apply ObsEq.coinductWith (fun -/
-  /-   (iTree.mk (State := State₁) curr₁ step₁) -/
-  /-   (iTree.mk (State := State₂) curr₂ step₂) => -/
-  /-   ∃ (H : State₁ = (Unit ⊕ State₂)), -/
-  /-   curr₁ = H.mpr (Sum.inr curr₂) ∧ -/
-  /-   ∀ (s : State₂), -/
-  /-   step₁ (H ▸ (.inr s)) = H.symm ▸ (step₂ s).mapState .inr -/
-  /- ) -/
-  /- case baseCase => -/
-  /-   simp [tau, Obs.mapState] -/
-  /- case progress => -/
-  /-   unfold func ObsRel.func unfold -/
-  /-   rintro ⟨c₁, s₁⟩ ⟨c₂, s₂⟩ ⟨rfl, HC, Hs⟩ -/
-  /-   cases _ : s₁ c₁ <;> -/
-  /-   cases _ : s₂ c₂ <;> -/
-  /-   simp [*, Obs.mapState] -/
+    rintro it₁ it₂ ⟨H, HC, Hs⟩
+    cases h : it₁.step it₁.curr <;> simp only [h, unfold, HC, Hs, Obs.mapState]
+    case ret v => 
+      constructor; rfl
+    case tau it => 
+      constructor
+      exists H
+    case vis ev k => 
+      constructor
+      intros
+      exists H
 
 theorem ObsEq.tau_congr {it₁ it₂ : iTree E R} : it₁ ≈ it₂ → (iTree.tau it₁) ≈ (iTree.tau it₂) := by
   intro h
-  unfold Rel
-  simp [unfold, tau, ObsRel]
+  unfold StrongBisim
+  simp [unfold, tau]
+  constructor
   change ({ it₁.tau with curr := .inr it₁.curr } ≈ { it₂.tau with curr := .inr it₂.curr })
   calc { it₁.tau with curr := .inr it₁.curr }
-    _ ≈ (it₁ : iTree E R) := step_tau_obsEq_self ..
+    _ ≈ (it₁ : iTree E R) := (step_tau_obsEq_self ..).symm
     _ ≈ it₂ := h
-    _ ≈ { it₂.tau with curr := .inr it₂.curr } := (step_tau_obsEq_self ..).symm
-
-theorem ObsEq.obsEq_ret_of_unfold_ret {it : iTree E R} {v : R} : it.unfold = .ret v → it ≈ .ret v := by
-  simp [unfold]
-  cases h : it.step it.curr <;> simp
-  rintro rfl
-  unfold Rel ObsRel unfold
-  simp [h, ret]
-
-theorem ObsEq.obsEq_tau_of_unfold_tau {it it': iTree E R} : it.unfold = .tau it' → it ≈ .tau it' := by
-  simp [unfold]
-  cases h : it.step it.curr <;> simp
-  case tau st =>
-    rintro rfl
-    unfold Rel ObsRel unfold
-    have := step_tau_obsEq_self it st st |>.symm
-    simpa [tau, h]
-
-theorem ObsEq.obsEq_tau_of_obsEq_unfold_tau {it it'₁ it'₂ : iTree E R} :
-    it.unfold = .tau it'₁ →
-    it'₁ ≈ it'₂ →
-    it ≈ .tau it'₂ := by
-  simp [unfold]
-  cases h : it.step it.curr <;> simp
-  case tau st =>
-  rintro rfl heq
-  have := ObsEq.tau_congr heq
-  refine ObsEq.trans ?_ this
-  unfold Rel ObsRel unfold
-  simpa [*, tau] using ObsEq.step_tau_obsEq_self it st st |>.symm
-
-theorem ObsEq.obsEq_vis_of_unfold_vis {it : iTree E R}{ev : E A} {k}: it.unfold = .vis ev k → it ≈ .vis ev k := by
-  simp [unfold]
-  cases h : it.step it.curr <;> simp
-  case vis A ev kS =>
-    rintro rfl rfl rfl
-    unfold Rel ObsRel unfold
-    simp [vis, h]
-    intros a
-    /- have := ObsEq.step_vis_obsEq_self it ev kS a -/
-    /- dsimp [HasEquiv.Equiv, instHasEquiv, ObsEq] at this -/
-    /- assumption -/
-    -- TODO: Idk why I can't conclude with the previous, so I just copy-paste the proof
-    -- of `ObsEq.step_vis_obsEq_self`
-    apply ObsEq.coinductWith (fun
-      (iTree.mk (State := State₁) curr₁ step₁)
-      (iTree.mk (State := State₂) curr₂ step₂) =>
-      ∃ (mpr : PUnit ⊕ (_ : A) × State₁ → State₂),
-      curr₂ = mpr (Sum.inr ⟨a, curr₁⟩) ∧
-      ∀ (s : State₁),
-      step₂ (mpr (.inr ⟨a, s⟩)) = (step₁ s).mapState (mpr <| .inr ⟨a, ·⟩)
-    )
-    case baseCase =>
-      exists id
-      simp [Obs.mapState]
-    case progress =>
-      rintro ⟨c₁, s₁⟩ ⟨c₂, s₂⟩ ⟨h, HC, Hs⟩
-      unfold ObsEq.func ObsRel.func unfold
-      cases _ : s₁ c₁ <;>
-      cases _ : s₂ c₂ <;>
-      simp [*, Obs.mapState]
-      all_goals (intros; exists h)
+    _ ≈ { it₂.tau with curr := .inr it₂.curr } := (step_tau_obsEq_self ..)
 
 theorem ObsEq.unfold_vis (ev : E A) (k : A → iTree E R) :
-    ObsRel (·=·) (iTree.vis ev k).unfold (Obs.vis ev k) := by
-  simp [unfold, iTree.vis, ObsRel]
+    (iTree.vis ev k).unfold ≈ (Obs.vis ev k) := by
+  simp [unfold, iTree.vis]
+  refine RelOverObs.vis _ _ _ _ ?_
   intro a
-  apply ObsEq.coinductWith (fun
+  apply coinductOn (fun
     (iTree.mk (State := State₂) curr₂ step₂)
     (iTree.mk (State := State₁) curr₁ step₁) =>
     ∃ (mpr : (Unit ⊕ (_ : A) × State₁) → State₂),
@@ -899,15 +686,94 @@ theorem ObsEq.unfold_vis (ev : E A) (k : A → iTree E R) :
     simp
     exists (fun | .inl .unit => .inl .unit
                 | .inr ⟨_, st⟩ => .inr ⟨a, st⟩ )
-    simp [Obs.mapState]
+    simp only [implies_true, and_self]
   case progress =>
-    rintro ⟨c₁, s₁⟩ ⟨c₂, s₂⟩ ⟨h, HC, Hs⟩-- ⟨h, HC, Hs⟩
-    unfold ObsEq.func ObsRel.func unfold
-    cases h₁ : s₁ c₁ <;>
-    cases h₂ : s₂ c₂ <;>
-    simp [*, Obs.mapState]
-    all_goals (intros; exists h)
+    rintro it₁ it₂ ⟨H, HC, Hs⟩
+    cases h : it₂.step it₂.curr <;> simp only [h, unfold, HC, Hs, Obs.mapState]
+    case ret v => 
+      constructor; rfl
+    case tau it => 
+      constructor
+      exists H
+    case vis ev k => 
+      constructor
+      intros
+      exists H
 
+      
+theorem ObsEq.obsEq_ret_of_unfold_ret {it : iTree E R} {v : R} : it.unfold = .ret v → it ≈ .ret v := by
+  simp [unfold]
+  cases h : it.step it.curr <;> simp
+  rintro rfl
+  unfold StrongBisim
+  simp only [h, unfold, ret]
+  constructor; rfl
+
+theorem ObsEq.obsEq_tau_of_unfold_tau {it it': iTree E R} : it.unfold = .tau it' → it ≈ .tau it' := by
+  simp [unfold]
+  cases h : it.step it.curr <;> simp
+  case tau st =>
+    rintro rfl
+    simp [tau] at *
+    apply coinductOn (fun
+      (iTree.mk (State := State₁) curr₁ step₁)
+      (iTree.mk (State := State₂) curr₂ step₂) =>
+      ∃ (mpr : (PUnit ⊕ State₁) → State₂),
+      step₂ curr₂ = (step₁ curr₁).mapState (mpr <| .inr ·) ∧
+      ∀ (s : State₁),
+      step₂ (mpr (.inr s)) = (step₁ s).mapState (mpr <| .inr ·)
+    )
+    case baseCase =>
+      simp
+      exists id
+      simp only [id_eq, implies_true, and_true, h]
+    case progress =>
+      rintro it₁ it₂ ⟨H, Hc, Hs⟩
+      cases h : it₁.step it₁.curr <;> simp only [h, unfold, Hc, Obs.mapState]
+      case ret v => 
+        constructor; rfl
+      case tau it => 
+        constructor
+        exists H
+        simp [Hs]
+      case vis ev k => 
+        constructor
+        intros
+        exists H
+        simp [Hs]
+
+theorem ObsEq.obsEq_vis_of_unfold_vis {it : iTree E R}{ev : E A} {k}: it.unfold = .vis ev k → it ≈ .vis ev k := by
+  simp only [unfold]
+  cases h : it.step it.curr <;> simp [reduceCtorEq, false_implies]
+  case vis A ev kS =>
+    rintro rfl rfl rfl
+    unfold StrongBisim
+    simp only [unfold, h, vis]
+    apply RelOverObs.vis _ _ _ _ ?_
+    intro a
+    apply ObsEq.coinductOn (fun
+      (iTree.mk (State := State₁) curr₁ step₁)
+      (iTree.mk (State := State₂) curr₂ step₂) =>
+      ∃ (mpr : PUnit ⊕ (_ : A) × State₁ → State₂),
+      curr₂ = mpr (Sum.inr ⟨a, curr₁⟩) ∧
+      ∀ (s : State₁),
+      step₂ (mpr (.inr ⟨a, s⟩)) = (step₁ s).mapState (mpr <| .inr ⟨a, ·⟩)
+    )
+    case baseCase =>
+      exists id
+      simp [Obs.mapState]
+    case progress =>
+      rintro ⟨c₁, s₁⟩ ⟨c₂, s₂⟩ ⟨H, HC, Hs⟩
+      cases h : s₁ c₁ <;> simp only [h, unfold, HC, Hs, Obs.mapState]
+      case ret v => 
+        constructor; rfl
+      case tau it => 
+        constructor
+        exists H
+      case vis ev k => 
+        constructor
+        intros
+        exists H
 
 def iTree.obsEqElim {motive : iTree E R → Type _}
   (inv : ∀ {it it'}, it ≈ it' → motive it' → motive it)
@@ -924,9 +790,9 @@ def iTree.obsEqElim {motive : iTree E R → Type _}
     exact inv (ObsEq.obsEq_vis_of_unfold_vis h) (vis ..)
 
 instance instEquiv  : Equivalence (fun (x y : iTree E R) => x ≈ y) where
-  refl  := Std.Refl.refl
-  symm  := Std.Symm.symm _ _
-  trans := Trans.trans
+  refl _ := StrongBisim.refl
+  symm   := StrongBisim.symm
+  trans  := StrongBisim.trans
 
 instance instSetoid : Setoid (iTree E R) where
   r := ObsEq
@@ -946,38 +812,28 @@ def unfold (it' : iTree' E R) : Obs E R (iTree' E R) :=
   it'.lift (fun it =>
     it.unfold.mapState iTree'.mk
   ) (by
-    intros it₁ it₂ heq
-    match h₁ : it₁.unfold, h₂ : it₂.unfold with
-    | Obs.ret _, Obs.ret _ =>
-      simp [h₁, h₂]
-      grind only [ObsEq.unfold_eq_ret]
-    | Obs.vis (A := A₁) ev₁ k₁, Obs.vis (A := A₂) ev₂ k₂ =>
-      simp [*, Obs.mapState]
-      obtain ⟨rfl, rfl, ih⟩:= ObsEq.unfold_eq_vis h₁ h₂ heq
-      simp only [heq_eq_eq, true_and]
-      ext
-      apply Quotient.sound
-      apply ih
-    | Obs.tau it₁', Obs.tau it₃' =>
-      simp [*, Obs.mapState]
-      apply Quotient.sound
-      apply ObsEq.unfold_eq_tau h₁ h₂ heq
-    | .ret .., .tau ..
-    | .ret .., .vis ..
-    | .vis .., .ret ..
-    | .vis .., .tau ..
-    | .tau .., .vis ..
-    | .tau .., .ret .. =>
-      grind)
+    intros it₁ it₂ it₁it₂
+    match StrongBisim.cases <| it₁it₂ with 
+    | ⟨.ret v₁, .ret v₂, h₁, h₂, .ret _ _ h⟩ =>
+      simp only [Obs.mapState, h₁, h₂, h]
+    | ⟨.tau it₁, .tau it₂, h₁, h₂, .tau _ _ h⟩ =>
+      simp only [Obs.mapState, Obs.tau.injEq, h₁, h₂]
+      apply Quotient.sound h
+    | ⟨.vis ev k₁, .vis _ k₂, h₁, h₂, .vis _ _ _ _ hK⟩ =>
+      simp [*]
+      ext a
+      apply Quotient.sound (hK a)
+  )
 
+-- picks an element out of the quotient, but bumps up the universes
 def out (it' : iTree' E R) : iTree E R where
     curr := it'
     step := iTree'.unfold
 
-theorem unfold_out (it' : iTree' E R) :
-    ObsRel (·=·) (it'.unfold.mapState (·.out)) (it'.out.unfold) :=
+/- theorem unfold_out (it' : iTree' E R) : -/
+/-     ObsRel (·=·) (it'.unfold.mapState (·.out)) (it'.out.unfold) := -/
   -- Basically, we can unfold either in the quotient our outside of it
-    sorry
+    /- sorry -/
 /-   apply it'.ind -/
 /-   intros it -/
 /-   cases h: it.unfold <;> -/
@@ -1009,13 +865,14 @@ theorem unfold_eq_tau (it' it'₂ : iTree' E R) :
   apply it'.ind; intros it
   apply it'₂.ind; intro it₂
   intros h
-  simp [tau, Quotient.lift, Quotient.mk]
+  simp only [tau, Quotient.lift, Quotient.mk]
   apply Quotient.sound
   simp [unfold, Quotient.lift, Quotient.mk, Obs.mapState] at h
   cases h₂ : it.unfold <;> simp [h₂] at h
   case a.tau it₂ =>
     have h := Quotient.exact h
-    apply ObsEq.obsEq_tau_of_obsEq_unfold_tau h₂ h
+    refine .trans ?_ (ObsEq.tau_congr h)
+    apply ObsEq.obsEq_tau_of_unfold_tau h₂
 
 -- def vis {A : Type a} {R : Type _}{E : Type a → Type _} (ev : E A) (k' : A → iTree' E R) : iTree' E R :=
 --   let k := fun a =>
@@ -1038,6 +895,8 @@ theorem unfold_eq_tau (it' it'₂ : iTree' E R) :
 --   case a.tau it₂ =>
 --     have h := Quotient.exact h
 --     apply ObsEq.obsEq_tau_of_obsEq_unfold_tau h₂ h
+
+section doubious
 
 instance piSetoid {ι : Sort _} {α : ι → Sort _} [∀ i, Setoid (α i)] : Setoid (∀ i, α i) where
   r a b := ∀ i, a i ≈ b i
@@ -1065,23 +924,17 @@ noncomputable
 def _root_.Quotient.bubbleUp{X A : Type _}{s : Setoid X}(f : A → Quotient s) : Quotient (piSetoid : Setoid (A → X)) :=
   Quotient.choice (ι := A) (α := λ_↦X) (S := λ_↦s) f
 
+end doubious
+
 
 
 def vis {A : Type a} {R : Type _}{E : Type a → Type _} (ev : E A) (k' : A → iTree' E R) : iTree' E R :=
   (Quotient.bubbleUp k').lift (.mk <| iTree.vis ev ·) (
     fun k₁ k₂ k₁k₂ =>
     Quotient.sound <| by
-    change ObsEq (iTree.vis ev k₁) (iTree.vis ev k₂)
-    unfold ObsEq Rel
-    have h₁ := ObsEq.unfold_vis ev k₁
-    have h₂ := ObsEq.unfold_vis ev k₂
-    have : ObsRel (·=·) (Obs.vis ev k₁) (Obs.vis ev k₂) := by
-      unfold ObsRel
-      exists rfl
+    -- I need some kind of congruence lemma for `iTree.tau`
     sorry -- TODO: Put it all together, may need to define symm and trans for `ObsRel`.
   )
-
-
 
 def elim {R : Type r}{E : Type a → Type e} {motive : iTree' E R → Type _}
   (ret : (v : R) → motive (.ret v))
@@ -1094,65 +947,7 @@ end iTree'
 
 end ThirdTry
 
-export SecondTry (eq wb wb.ret wb.vis wb.tauL wb.tauR wb.sync)
-
 end EqualitiesOverITrees
-
-@[simp, grind]
-instance : HasEquiv (iTree E R) where Equiv := SecondTry.eq
-
--- This definition doesn't satisfy the monad laws up to equality, but it does
--- follow then up to tau equality.
-
-/- theorem bindLeft_ret : it.unfold = .ret v → bindLeft f it = sorry := by -/
-/-   intros h -/
-/-   unfold bindLeft -/
-/-   sorry -/
-
-
-theorem id_map {α : Type} (it : iTree E α) : bindLeft pure it ≈ it := by
-  dsimp [HasEquiv.Equiv]
-  unfold eq
-  match h : it.unfold with
-  | .ret v₁ =>
-    cases h₂ : it.step it.curr <;> (try simp [h₂, unfold] at h; done)
-    apply wb.tauL ?_ ?unfold ?next
-    case unfold =>
-      simp [unfold, bindLeft, h₂, Obs.bindVal, Obs.mapState]
-      rfl
-    apply wb.ret v₁ _ h
-    simp [unfold, pure, ret]
-    simp [unfold, h₂] at h
-    assumption
-  | .vis ev₁ k₁ =>
-    cases h₂ : it.step it.curr <;> (try simp [h₂, unfold] at h; done)
-    case vis A ev₁ k₁ =>
-    /- have := h -/
-    simp [h₂, unfold] at h
-    have ⟨rfl, h⟩ := h
-    simp at h
-    have ⟨h, h'⟩:= h
-    subst h h'
-    simp [bindLeft,  Obs.bindVal, Obs.mapState]
-    apply wb.vis ev₁ _ ev₁ _ ?left ?right
-    case left =>
-      simp [unfold, h₂, pure, ret]
-      sorry
-    all_goals sorry
-  | .tau it₁ =>
-    sorry
-
-instance  : LawfulMonad (iTree E) := .mk'
-   (id_map     := by
-      simp only [Functor.map, bind, Pure.pure, Function.comp_id]
-      intros α it
-      have {State, curr, step} := it
-      simp [bindLeft, *]
-      sorry
-      /- induction it <;> simp [bindLeft, *] -/
-    )
-   (pure_bind  := by intros α β it f; simp only [bind, bindLeft])
-   (bind_assoc := by intros α β γ it f g; simp only [bind]; induction it <;> simp [bindLeft, *])
 
 end iTree
 
